

\subsection{\textit{Parseval's Theorem}}

	\textit{Parseval's Theorem states is a result of the Fourier Transform. It states that, the integral of the square of a function is equal to the sum of the square of its transform. Mathematically,}
	
		$$\frac{1}{\pi}\cdot\int_{-\pi}^{+\pi} \left(f(x)\right)^2 dx = \sum_{n=0}^{\infty}\left(a_{n}^2 + b_{n}^2\right)$$

	\textit{Conversely, could be generalized as,}

		$$\frac{1}{L}\cdot\int_{L} f^2(x) dx = \sum_{n=0}^{\infty}\left(a_{n}^2 + b_{n}^2\right)$$



